Add specs for Read and Write

src/Dafny/jrnl.i.dfy
@@ -4,8 +4,21 @@ datatype Addr = Addr(blkno: nat, off: nat)
 type byte = bv8
 type Object = array<byte>
 type Kind = k:int | 0 <= k <= 15
-function kindSize(k: Kind): int {
+
+function kindSize(k: Kind): nat {
+    pow_nonneg(2, k);
     pow(2,k)
+}
+
+function kindCount(k: Kind): nat {
+    pow_nonneg(2, 15-k);
+    pow(2, 15-k)
+}
+
+lemma kindSize_and_kindCount_sensible(k: Kind)
+ensures kindSize(k) * kindCount(k) == 4096*8 {
+    assert 4096*8 == pow(2, 15);
+    pow_plus(2, k, 15-k);
 }
 
 lemma kindSize_bounds(k: Kind)
@@ -14,13 +27,68 @@ ensures kindSize(k) <= 4096*8 {
     assert pow(2,15) == 4096*8;
 }
 
-class Jrnl {
-    ghost var data: map<Addr, Object>;
-    ghost var kinds: map<nat, Kind>;
+class {:autocontracts} Jrnl {
+    var data: map<Addr, Object>;
+    var kinds: map<nat, Kind>;
 
     predicate Valid() reads this {
         forall a :: a in data ==>
         && a.blkno in kinds
-        && data[a].Length == kindSize(kinds[a.blkno])
+        && data[a].Length*8 == kindSize(kinds[a.blkno])
+    }
+
+    constructor(kinds: map<nat, Kind>)
+    {
+        this.kinds := kinds;
+        // TODO: initializing data based on kinds is quite difficult
+        assume false;
+    }
+
+    function domain(): set<Addr>
+    {
+        set a:Addr | a in this.data
+    }
+
+    function size(a: Addr): nat
+    requires a in this.domain()
+    {
+        kindSize(this.kinds[a.blkno])
+    }
+
+    method Begin() returns (txn:Txn)
+    {
+        return new Txn(this);
+    }
+}
+
+class Txn {
+    var jrnl: Jrnl;
+
+    constructor(jrnl: Jrnl)
+    requires jrnl.Valid()
+    {
+        this.jrnl := jrnl;
+    }
+
+    predicate Valid() reads {this,this.jrnl} + this.jrnl.Repr {
+        this.jrnl.Valid()
+    }
+
+    method Read(a: Addr, sz: nat)
+    returns (o:Object)
+    requires this.Valid()
+    requires a in this.jrnl.domain()
+    requires sz == this.jrnl.size(a)
+    {
+        return this.jrnl.data[a];
+    }
+
+    method Write(a: Addr, obj: Object)
+    modifies this.jrnl
+    requires this.Valid()
+    requires a in this.jrnl.domain()
+    requires obj.Length*8 == this.jrnl.size(a)
+    {
+        this.jrnl.data := this.jrnl.data[a:=obj];
     }
 }
