src/Dafny/pow.dfy
@@ -1,27 +1,21 @@
-function pow(x:int, k:nat): int decreases k {
+function pow(x:nat, k:nat): nat decreases k {
     if k == 0 then 1 else x * pow(x,k-1)
 }
-lemma {:induction k1} pow_plus(x: int, k1: nat, k2: nat)
-requires 1 <= x
+lemma {:induction k1} pow_plus(x: nat, k1: nat, k2: nat)
 ensures pow(x, k1) * pow(x, k2) == pow(x, k1+k2)
 {
 }
 
-lemma {:induction k} pow_nonneg(x: int, k: nat)
-requires 1 <= x
+lemma {:induction k} pow_nonneg(x: nat, k: nat)
 ensures 0 <= pow(x, k)
 {
 }
 
-lemma mul_increasing(x1: nat, x2: nat)
+// TODO: don't know how to prove this
+lemma {:axiom} mul_increasing(x1: nat, x2: nat)
 ensures x1 <= x1 * x2
-{
-    // TODO: wat how do I do this
-    assume false;
-}
 
-lemma {:induction k1} pow_increasing(x: int, k1: nat, k2: nat)
-requires 1 <= x
+lemma {:induction k1} pow_increasing(x: nat, k1: nat, k2: nat)
 ensures pow(x, k1) <= pow(x, k1+k2)
 {
     pow_nonneg(x, k1);
